Memory/Error.v
@@ -1,0 +1,38 @@
+Require Import String.
+
+Close Scope string_scope.
+
+Declare Scope error_monad_scope.
+
+Set Implicit Arguments.
+
+(** Error Monad *)
+
+Inductive result (A: Type) : Type :=
+| Ok: A -> result A
+| Error: string -> result A.
+
+Arguments Error [A].
+
+Definition bind (A B: Type) (f: result A) (g: A -> result B) : result B :=
+  match f with
+  | Ok x => g x
+  | Error msg => Error msg
+  end.
+
+Definition bind2 (A B C: Type) (f: result (A*B)) (g: A->B->result C) : result C :=
+  match f with
+  | Ok (x, y) => g x y
+  | Error msg => Error msg
+  end.
+
+Notation "'do' X <- A ; B" := (bind A (fun X => B))
+ (at level 200, X name, A at level 100, B at level 200)
+ : error_monad_scope.
+
+Notation "'do' ( X , Y ) <- A ; B" := (bind2 A (fun X Y => B))
+ (at level 200, X name, Y name, A at level 100, B at level 200)
+ : error_monad_scope.
+
+Definition lift (A B: Type)(f:A->B): result A -> result B :=
+  fun x => bind x (fun v => Ok (f v)).
