Memory/Option.v
@@ -1,8 +1,35 @@
 Notation "'⎣' v '⎦'" := (Some v).
 Notation "'ϵ'" := (None).
 
+Declare Scope option_monad_scope.
+
 Definition is_ϵ {A} (v: option A) :=
   match v with
   | ϵ => true
   | _ => false
   end.
+
+Set Implicit Arguments.
+
+Definition bind (A B: Type) (f: option A) (g: A -> option B) : option B :=
+  match f with
+  | Some x => g x
+  | None => None
+  end.
+
+Definition bind2 (A B C: Type) (f: option (A*B)) (g: A->B->option C) : option C :=
+  match f with
+  | Some (x, y) => g x y
+  | None => None
+  end.
+
+Notation "'do' X <- A ; B" := (bind A (fun X => B))
+ (at level 200, X name, A at level 100, B at level 200)
+ : option_monad_scope.
+
+Notation "'do' ( X , Y ) <- A ; B" := (bind2 A (fun X Y => B))
+ (at level 200, X name, Y name, A at level 100, B at level 200)
+ : option_monad_scope.
+
+Definition lift (A B: Type)(f:A->B): option A -> option B :=
+  fun x => bind x (fun v => Some (f v)).
