Memory/Semantics.v
@@ -1,0 +1,147 @@
+Require Import Arith ZArith Lia List Structures.Equalities.
+Require Import Vrac.Tactics Vrac.Option Vrac.Eqb Vrac.MemoryType
+  Vrac.ExecutionMemoryModel Vrac.Context Vrac.Syntax Vrac.Error.
+
+Module Semantics(V : DecidableType)(B: Eqb.EQB)
+  (Import EMM: ExecutionMemoryModel B)
+  (Import Ctx: Context.SIG V B EMM)
+  (Import Stx: Syntax.SIG V).
+
+  Import Stx.Types.
+
+  Definition mtype := mtype machine_word.
+  
+  Inductive kind := KInt | KPtr | KUn.
+  
+  Definition kind_t (τ : type) : kind :=
+    match τ with
+    | TInt _ => KInt
+    | TPtr _ => KPtr
+    end.
+
+  Definition kind_v (v : value) : kind :=
+    match v with
+    | Int _ => KInt
+    | Ptr _ => KPtr
+    | _ => KUn
+    end.
+
+  Definition valid_expr (Γ: type_env)(e: Stx.expr) : Prop :=
+    exists τ, check_type Γ e = Ok τ.
+
+  Ltac rewrite_clear :=
+    match goal with
+    | [ H: _ = _ |- _ ] =>
+        try rewrite H; clear H
+    end.
+
+  Ltac check_type :=
+    intros; simpl; repeat rewrite_clear; simpl;
+    unfold same_as_checked; now simpl_type_eqb.
+  
+  Fact deref_check_type:
+    forall Γ e τ,
+    check_type Γ e = Ok (TPtr τ) ->
+    check_type Γ (EDeref e τ) = Ok τ.
+  Proof. check_type. Qed.
+  
+  Fact parith_check_type:
+    forall Γ e1 τ1 e2 κ2,
+      check_type Γ e1 = Ok (TPtr τ1) ->
+      check_type Γ e2 = Ok (TInt κ2) ->
+      check_type Γ (EBinop Oadd e1 e2 (TPtr τ1)) = Ok (TPtr τ1).
+  Proof. check_type. Qed.
+
+  Inductive eeval: Ctx.context -> Stx.type_env -> Stx.expr -> value -> Prop :=
+  | E_int: forall C Γ n τ,
+      valid_expr Γ (EInt n τ) ->
+      eeval C Γ (EInt n τ) (Int n)
+  | E_addr: forall C Γ e τ b δ,
+      valid_expr Γ e ->
+      lveval C Γ e (b,δ) ->
+      eeval C Γ (EAddrof e τ) (Ptr(b,δ))
+  | E_lval: forall C Γ e τ b δ v,
+      check_type Γ e = Ok τ -> 
+      lveval C Γ e (b,δ) ->
+      EMM.load(mtype τ, C.(M), b, δ) = ⎣v⎦ ->
+      v <> Undef ->
+      kind_t τ = kind_v v ->
+      eeval C Γ e v
+  | E_parith: forall C Γ e1 τ1 v1 e2 κ2 b δ n sz e v,
+      check_type Γ e1 = Ok (TPtr τ1) ->
+      check_type Γ e2 = Ok (TInt κ2) ->
+      eeval C Γ e1 v1 -> v1 = (Ptr(b,δ)) ->
+      eeval C Γ e2 (Int n) ->
+      sz = sizeof(mtype τ1) ->
+      (δ mod sz = 0)%Z ->
+      e = EBinop Oadd e1 e2 (TPtr τ1) ->
+      v = Ptr(b,(δ+n*sz)%Z) ->
+      eeval C Γ e v
+  with lveval: Ctx.context -> Stx.type_env -> Stx.expr -> B.t * Z -> Prop :=
+  | LV_var: forall C Γ x τ b,
+      lveval C Γ (EVar x τ) (b,0%Z)
+  | LV_deref: forall C Γ e τ b δ,
+      check_type Γ e = Ok (TPtr τ) ->
+      eeval C Γ e (Ptr(b,δ)) ->
+      lveval C Γ (EDeref e τ) (b,δ)
+  .
+
+  Scheme eeval_ind' :=
+    Induction for eeval Sort Prop
+      with lveval_ind' :=
+      Induction for lveval Sort Prop.
+
+  Fact induced_undef:
+    forall σ Hσ v, v<>Undef -> induced σ Hσ v <> Undef.
+  Proof.
+    intros σ Hσ [n|[b δ]|] H; simpl;
+      try discriminate.
+    now contradict H.
+  Qed.
+
+  Fact induced_kind:
+    forall σ Hσ v, kind_v v = kind_v (induced σ Hσ v).
+  Proof.
+    intros σ Hσ [n|[b δ]|]; trivial.
+  Qed.
+  
+  Lemma isomorphic_evalexpr:
+    forall C C' Γ σ Hσ,
+      isomorphic C C' σ Hσ ->
+      (forall e v,
+          eeval C Γ e v ->
+          eeval C' Γ e (induced σ Hσ v)).
+  Proof.
+    intros C C' Γ σ Hσ Hiso e v Heeval.
+    generalize dependent C'. generalize dependent σ.
+    induction Heeval
+      using eeval_ind'
+      with (P0:=fun C Γ e ptr (H: lveval C Γ e ptr) =>
+                  forall C' σ Hσ (Hiso: isomorphic C C' σ Hσ),
+                    let (b,δ) := ptr in
+                    lveval C' Γ e (σ b, δ)); subst.
+    - intros. now constructor.
+    - constructor.
+      + trivial.
+      + eapply IHHeeval; eauto.
+    - intros σ Hσ C' Hiso.
+      assert(Hlveval: lveval C' Γ e (σ b, δ)) by eauto.
+      assert(Hload: load (mtype τ, C'.(M), σ b, δ) = ⎣ induced σ Hσ v ⎦)
+        by now rewrite <- iso_load.
+      eapply E_lval; eauto.
+      + now apply induced_undef.
+      + now rewrite <- induced_kind.
+    - simpl in *.
+      intros σ Hσ C' Hiso.
+      specialize (IHHeeval1 σ Hσ C' Hiso).
+      specialize (IHHeeval2 σ Hσ C' Hiso).
+      eapply E_parith; eauto.
+    - intros; constructor.
+    - intros C' σ Hσ Hiso. simpl in *.
+      econstructor; eauto.
+  Qed.
+
+End Semantics.
+
+
+
