Memory/Syntax.v
@@ -1,0 +1,138 @@
+Require Import ZArith Structures.Equalities String.
+Require Import Vrac.MemoryType Vrac.Error Vrac.Option Vrac.Tactics.
+
+
+
+Module Syntax(V : DecidableType).
+
+  Module Types.
+  
+    Inductive type :=
+    | TInt : Mtyp.t -> type
+    | TPtr: type -> type.
+
+    Definition t := type.
+    
+    Definition mtype: mtyp -> type -> mtyp :=
+      fun machine_word ty =>
+        match ty with
+        | TInt mtype => mtype 
+        | TPtr _ => machine_word
+        end.
+
+    Fixpoint eqb τ1 τ2 : bool :=
+      match (τ1, τ2) with
+      | (TInt κ1, TInt κ2) => Mtyp.eqb κ1 κ2
+      | (TPtr τ'1, TPtr τ'2) => eqb τ'1 τ'2
+      | _ => false
+      end.
+
+    Lemma eqb_eq : forall x y, eqb x y = true <-> x = y.
+    Proof.
+      intros x y; split; intro H; revert H; revert y.
+      - induction x as [|x Hx]; destruct y;
+          intro H; simpl in *; try discriminate.
+        + apply Mtyp.eqb_eq in H.
+          now subst.
+        + apply Hx in H.
+          now subst.
+      - induction x as [|x Hx]; destruct y;
+          intro H; simpl in *; try discriminate.
+        + inversion H; subst.
+          now simpl_mtyp_eqb.
+        + apply Hx.
+          now inversion H.
+    Qed.
+
+  End Types.
+  
+  Module T := Eqb.Full Types. Import Types. Import T.
+
+  Ltac simpl_type_eqb :=
+    simpl_generic_eqb eqb eqb_refl eqb_sym eqb_eq eqb_neq.
+  
+  Inductive unary_operation : Type :=
+  | Onot
+  | Oneg.
+  
+  Inductive binary_operation : Type :=
+  | Oadd  (* addition *)
+  | Osub  (* subtraction *)
+  | Omul  (* multiplication *)
+  | Odiv  (* division *)
+  | Omod  (* remainder *)
+  | Oeq   (* comparison (==) *)
+  | Olt   (* comparison (<) *)
+  | Ogt   (* comparison (>) *)
+  | Ole   (* comparison (<=) *)
+  | Oge   (* comparison (>=) *).
+
+  Inductive expr : Type :=
+  | EInt (n: Z) (τ: type)      (* Integer value *)
+  | EVar (x: V.t) (τ: type)    (* variable *)
+  | EDeref (e: expr) (τ: type) (* dereference *)
+  | EAddrof (e: expr) (τ: type)(* address *)
+  | EUnop (op: unary_operation) (e: expr) (τ: type)
+  | EBinop (op: binary_operation) (e1 e2: expr) (τ: type).
+
+  Definition type_int (n:Z) (τ:type) : result type :=
+    match τ with
+    | TInt κ =>  if ( (min_int (sizeof κ)<=? n)%Z &&
+                     (n <=? max_int (sizeof κ))%Z )%bool
+                then Ok τ
+                else Error "not storable"
+    | _ => Error "not an integer type"
+    end.
+
+  Open Scope error_monad_scope.
+
+  Definition same_as_checked τ τ' : result type :=
+     if Types.eqb τ τ'
+     then Ok τ
+     else Error "type mismatch".
+
+  Definition type_env := V.t -> option type.
+  
+  Fixpoint check_type (Γ: type_env) (e: expr) : result type :=
+    match e with
+    | EInt n τ => type_int n τ
+    | EVar x τ => match Γ x with
+                 | ϵ => Error "undefined identifier"
+                 | ⎣τ'⎦ => same_as_checked τ τ'
+                 end
+    | EDeref e τ =>
+        match check_type Γ e with 
+        | Ok (TPtr τ') => same_as_checked τ τ'
+        | _ => Error "not dereferencing a pointer"
+        end
+    | EAddrof e τ =>
+        do τ' <- check_type Γ e;
+        same_as_checked τ (TPtr τ')
+    | EUnop op e τ =>
+        do τ' <- check_type Γ e;
+        match τ' with
+        | TInt _ => same_as_checked τ τ'
+        | TPtr _ => Error "no unary operation on pointers"
+        end
+    | EBinop op e1 e2 τ =>
+        do τ1 <- check_type Γ e1;
+        do τ2 <- check_type Γ e2;
+        match (op, τ1, τ2) with
+        | (_, TInt κ1, TInt κ2) =>
+            same_as_checked τ (TInt (MemoryType.max κ1 κ2))
+        | ((Oadd|Osub), TPtr τ', TInt _) =>
+            same_as_checked τ (TPtr τ')
+        | (Oeq, TPtr τ'1, TPtr τ'2) =>
+            if Types.eqb τ'1 τ'2
+            then same_as_checked τ (TInt i8)
+            else Error "incompatible types for eq"
+        | _ => Error "incorrect types for binary operation"
+        end
+    end.
+  
+End Syntax.
+
+Module Type SIG(V : DecidableType).
+  Include Syntax V.
+End SIG.
+
